\section{Calculations}

In the next steps of calculating the decay rates we will need some terms repeatedly. Therefore theses terms should be calculated here in a separated chapter
to keep the next parts then clearer. As this calculations here does not depend on any specific finalstate we don't distinguish between \Lf and
\Lfbar and just use a general parameter $\lambda$.

The first term we will need are
\begin{equation}
    e_{+}e_{-}^*\lambda^{\ast}+e_+^*e_-\lambda \hspace{0.5cm} \text{and} \hspace{0.5cm} e_{+}^*e_{-}\lambda^{\ast}+e_+e_-^*\lambda.
\end{equation}
To calculate these we start with writing down the full expressions of $e_+$, $e_+^*$, $e_-$ and $e_-^*$ :
\begin{align}
  e_+ &= \frac{1}{2}\left(e^{\left(-im_{\text{H}}-\frac{1}{2}\Gamma_{\text{H}}\right)t}+e^{\left(-im_{\text{L}}-\frac{1}{2}\Gamma_{\text{L}}\right)t}\right)\\
  e_+^* &= \frac{1}{2}\left(e^{\left(im_{\text{H}}-\frac{1}{2}\Gamma_{\text{H}}\right)t}+e^{\left(im_{\text{L}}-\frac{1}{2}\Gamma_{\text{L}}\right)t}\right)\\
  e_- &= \frac{1}{2}\left(e^{\left(-im_{\text{H}}-\frac{1}{2}\Gamma_{\text{H}}\right)t}-e^{\left(-im_{\text{L}}-\frac{1}{2}\Gamma_{\text{L}}\right)t}\right)\\
  e_-^* &= \frac{1}{2}\left(e^{\left(im_{\text{H}}-\frac{1}{2}\Gamma_{\text{H}}\right)t}-e^{\left(im_{\text{L}}-\frac{1}{2}\Gamma_{\text{L}}\right)t}\right)
\end{align}
Now we can compute the products of these exponential functions:
\begin{align}
    e_+e_-^* &=\frac{1}{4}\left(e^{-\Gamma_{\text{H}}t}-e^{\left(-im_{\text{H}}-\frac{1}{2}\Gamma_{\text{H}}+im_{\text{L}}-\frac{1}{2}\Gamma_{\text{L}}\right)t}
    +e^{\left(-im_{\text{L}}-\frac{1}{2}\Gamma_{\text{L}}+im_{\text{H}}-\frac{1}{2}\Gamma_{\text{H}}\right)}-e^{-\Gamma_{\text{L}}t}\right)\nonumber\\
    &= \frac{1}{4}\left(e^{-\Gamma_{\text{H}}t}-e^{-i\left(m_{\text{H}}-m_{\text{L}}\right)t}e^{-\frac{1}{2}\left(\Gamma_{\text{H}}+\Gamma_{\text{L}}\right)t}
    +e^{i\left(m_{\text{H}}-m_{\text{L}}\right)t}e^{-\frac{1}{2}\left(\Gamma_{\text{H}}+\Gamma_{\text{L}}\right)t}-e^{-\Gamma_{\text{L}}t}\right)\nonumber\\
    &=\frac{1}{4}\left(e^{-\Gamma_{\text{H}}t}-e^{-\Gamma_{\text{L}}t}+e^{-\Gamma t}\left(e^{i\Delta mt}-e^{-i\Delta mt}\right)\right)\nonumber\\
    &=\frac{1}{4}e^{-\Gamma t}\left(e^{\left(-\Gamma_{\text{H}}+\Gamma\right)t} - e^{\left(-\Gamma_{\text{L}}+\Gamma\right)t} + 2i\sin\left(\Delta m\right)\right)\nonumber\\
    &=\frac{1}{2}e^{-\Gamma t}\left(\frac{1}{2}e^{-\frac{\Gamma_{\text{H}}-\Gamma_{\text{L}}}{2}t} - \frac{1}{2}e^{\frac{\Gamma_{\text{H}}-\Gamma_{\text{L}}}{2}t}\right)
    +i\sin\left(\Delta m\right)\nonumber\\
    &= -\frac{1}{2}e^{-\Gamma t}\left(\frac{1}{2}\left(e^{\frac{\Delta\Gamma}{2}t} - e^{-\frac{\Delta\Gamma}{2}t}\right)
    -i\sin\left(\Delta m\right)\right)\nonumber\\
    &= -\frac{1}{2}e^{-\Gamma t}\left(\sinh\left(\frac{\Delta\Gamma}{2}t\right)-i\sin\left(\Delta m t\right)\right)\label{eq:first_calculation}\\
    e_+^*e_- &=\frac{1}{4}\left(e^{-\Gamma_{\text{H}}t}-e^{\left(im_{\text{H}}-\frac{1}{2}\Gamma_{\text{H}}-im_{\text{L}}-\frac{1}{2}\Gamma_{\text{L}}\right)t}
    +e^{\left(im_{\text{L}}-\frac{1}{2}\Gamma_{\text{L}}-im_{\text{H}}-\frac{1}{2}\Gamma_{\text{H}}\right)}-e^{-\Gamma_{\text{L}}t}\right)\nonumber\\
    &= \frac{1}{4}\left(e^{-\Gamma_{\text{H}}t}-e^{i\left(m_{\text{H}}-m_{\text{L}}\right)t}e^{-\frac{1}{2}\left(\Gamma_{\text{H}}+\Gamma_{\text{L}}\right)t}
    +e^{-i\left(m_{\text{H}}-m_{\text{L}}\right)t}e^{-\frac{1}{2}\left(\Gamma_{\text{H}}+\Gamma_{\text{L}}\right)t}-e^{-\Gamma_{\text{L}}t}\right)\nonumber\\
    &=\frac{1}{4}\left(e^{-\Gamma_{\text{H}}t}-e^{-\Gamma_{\text{L}}t}-e^{-\Gamma t}\left(e^{i\Delta mt}-e^{-i\Delta mt}\right)\right)\nonumber\\
    &=\frac{1}{4}e^{-\Gamma t}\left(e^{\left(-\Gamma_{\text{H}}+\Gamma\right)t} - e^{\left(-\Gamma_{\text{L}}+\Gamma\right)t} - 2i\sin\left(\Delta m\right)\right)\nonumber\\
    &=\frac{1}{2}e^{-\Gamma t}\left(\frac{1}{2}e^{-\frac{\Gamma_{\text{H}}-\Gamma_{\text{L}}}{2}t} - \frac{1}{2}e^{\frac{\Gamma_{\text{H}}-\Gamma_{\text{L}}}{2}t}\right)
    -i\sin\left(\Delta m\right)\nonumber\\
    &= -\frac{1}{2}e^{-\Gamma t}\left(\frac{1}{2}\left(e^{\frac{\Delta\Gamma}{2}t} - e^{-\frac{\Delta\Gamma}{2}t}\right)
    +i\sin\left(\Delta m\right)\right)\nonumber\\
    &= -\frac{1}{2}e^{-\Gamma t}\left(\sinh\left(\frac{\Delta\Gamma}{2}t\right)+i\sin\left(\Delta m t\right)\right)\label{eq:second_calculation}
\end{align}
Using \cref{eq:first_calculation} and \cref{eq:second_calculation} makes it now easy to get the first to results of this chapter:
\begin{align}
  e_{+}e_{-}^*\lambda^{\ast}+e_+^*e_-\lambda =& e_+e_-^*\left(\mathcal{Re}(\lambda)-i\mathcal{Im}(\lambda)\right)
  + e_+^*e_-\left(\mathcal{Re}(\lambda)+i\mathcal{Im}(\lambda)\right)\nonumber\\
  =& -\frac{1}{2}e^{-\Gamma t}\left[\left(\sinh\left(\frac{\Delta\Gamma}{2}t\right)-i\sin\left(\Delta m t\right)\right)\mathcal{Re}(\lambda)\right.\nonumber\\
  &-\left(\sinh\left(\frac{\Delta\Gamma}{2}t\right)-i\sin\left(\Delta m t\right)\right)i\mathcal{Im}(\lambda)\nonumber\\
  &+\left(\sinh\left(\frac{\Delta\Gamma}{2}t\right)+i\sin\left(\Delta m t\right)\right)\mathcal{Re}(\lambda)\nonumber\\
  &+\left.\left(\sinh\left(\frac{\Delta\Gamma}{2}t\right)+i\sin\left(\Delta m t\right)\right)i\mathcal{Im}(\lambda)\right]\nonumber\\
  =&-\frac{1}{2}e^{-\Gamma t}\left[2\sinh\left(\frac{\Delta\Gamma}{2}t\right)\mathcal{Re}(\lambda)-2\sin\left(\Delta mt\right)\mathcal{Im}(\lambda)\right]\nonumber\\
  =&-e^{-\Gamma t}\left[\sinh\left(\frac{\Delta\Gamma}{2}t\right)\mathcal{Re}(\lambda)-\sin\left(\Delta mt\right)\mathcal{Im}(\lambda)\right]\label{eq:result_1}\\
  e_{+}^*e_{-}\lambda^{\ast}+e_+e_-^*\lambda =& e_+^*e_-\left(\mathcal{Re}(\lambda)-i\mathcal{Im}(\lambda)\right)
  + e_+e_-^*\left(\mathcal{Re}(\lambda)+i\mathcal{Im}(\lambda)\right)\nonumber\\
  =& -\frac{1}{2}e^{-\Gamma t}\left[\left(\sinh\left(\frac{\Delta\Gamma}{2}t\right)+i\sin\left(\Delta m t\right)\right)\mathcal{Re}(\lambda)\right.\nonumber\\
  &-\left(\sinh\left(\frac{\Delta\Gamma}{2}t\right)+i\sin\left(\Delta m t\right)\right)i\mathcal{Im}(\lambda)\nonumber\\
  &+\left(\sinh\left(\frac{\Delta\Gamma}{2}t\right)-i\sin\left(\Delta m t\right)\right)\mathcal{Re}(\lambda)\nonumber\\
  &+\left.\left(\sinh\left(\frac{\Delta\Gamma}{2}t\right)-i\sin\left(\Delta m t\right)\right)i\mathcal{Im}(\lambda)\right]\nonumber\\
  =&-\frac{1}{2}e^{-\Gamma t}\left[2\sinh\left(\frac{\Delta\Gamma}{2}t\right)\mathcal{Re}(\lambda)+2\sin\left(\Delta mt\right)\mathcal{Im}(\lambda)\right]\nonumber\\
  =&-e^{-\Gamma t}\left[\sinh\left(\frac{\Delta\Gamma}{2}t\right)\mathcal{Re}(\lambda)+\sin\left(\Delta mt\right)\mathcal{Im}(\lambda)\right]\label{eq:result_2}
\end{align}
The next terms we will need are
\begin{equation}
  e_{+}e_{+}^*+\left|\lambda\right|^2e_-e_-^* \hspace{0.5cm} \text{and} \hspace{0.5cm} e_{+}e_{+}^*\left|\lambda\right|^2+e_-e_-^*.
\end{equation}
Again we compute first the products of the exponential functions:
\begin{align}
  e_+e_+^* &= \frac{1}{4}\left(e^{-\Gamma_{\text{H}}t}+e^{\left(-im_{\text{H}}-\frac{1}{2}\Gamma_{\text{H}}+im_{\text{L}}-\frac{1}{2}\Gamma_{\text{L}}\right)t}
  +e^{\left(-im_{\text{L}}-\frac{1}{2}\Gamma_{\text{L}}+im_{\text{H}}-\frac{1}{2}\Gamma_{\text{L}}\right)t}+e^{-\Gamma_{\text{L}}t}\right)\nonumber\\
  &= \frac{1}{4}\left(e^{-\Gamma_{\text{H}}t}+e^{-\Gamma_{\text{L}}t}+e^{-i\left(m_{\text{H}}-m_{\text{L}}\right)t}e^{-\frac{1}{2}\left(\Gamma_{\text{H}}+\Gamma_{\text{L}}\right)t}
  +e^{i\left(m_{\text{H}}-m_{\text{L}}\right)t}e^{-\frac{1}{2}\left(\Gamma_{\text{H}}+\Gamma_{\text{L}}\right)t}\right)\nonumber\\
  &=\frac{1}{4}e^{-\Gamma t}\left(e^{\left(-\Gamma_{\text{L}}+\Gamma\right)t}+e^{\left(-\Gamma_{\text{H}}+\Gamma\right)t}+2\cos\left(\Delta mt\right)\right)\nonumber\\
  &=\frac{1}{2}e^{-\Gamma t}\left(\frac{1}{2}e^{\frac{\Gamma_{\text{H}}-\Gamma_{\text{L}}}{2}t}+\frac{1}{2}e^{\frac{\Gamma_{\text{H}}-\Gamma_{\text{L}}}{2}t}+\cos\left(\Delta mt\right)\right)\nonumber\\
  &=\frac{1}{2}e^{-\Gamma t}\left(\cosh\left(\frac{\Gamma}{2}t\right)+\cos\left(\Delta mt\right)\right)\label{eq:third_calculation}\\
  e_-e_-^* &= \frac{1}{4}\left(e^{-\Gamma_{\text{H}}t}-e^{\left(-im_{\text{H}}-\frac{1}{2}\Gamma_{\text{H}}+im_{\text{L}}-\frac{1}{2}\Gamma_{\text{L}}\right)t}
  -e^{\left(-im_{\text{L}}-\frac{1}{2}\Gamma_{\text{L}}+im_{\text{H}}-\frac{1}{2}\Gamma_{\text{L}}\right)t}+e^{-\Gamma_{\text{L}}t}\right)\nonumber\\
  &= \frac{1}{4}\left(e^{-\Gamma_{\text{H}}t}+e^{-\Gamma_{\text{L}}t}-e^{-i\left(m_{\text{H}}-m_{\text{L}}\right)t}e^{-\frac{1}{2}\left(\Gamma_{\text{H}}+\Gamma_{\text{L}}\right)t}
  -e^{i\left(m_{\text{H}}-m_{\text{L}}\right)t}e^{-\frac{1}{2}\left(\Gamma_{\text{H}}+\Gamma_{\text{L}}\right)t}\right)\nonumber\\
  &= \frac{1}{2}e^{-\Gamma t}\left(\frac{1}{2}e^{\frac{\Gamma_{\text{H}}-\Gamma_{\text{L}}}{2}t}+\frac{1}{2}e^{\frac{\Gamma_{\text{H}}-\Gamma_{\text{L}}}{2}t}-\cos\left(\Delta mt\right)\right)\nonumber\\
  &= \frac{1}{2}e^{-\Gamma t}\left(\cosh\left(\frac{\Gamma}{2}t\right)-\cos\left(\Delta mt\right)\right)\label{eq:fourth_calculation}
\end{align}
Now using \cref{eq:third_calculation} and \cref{eq:fourth_calculation} the last two results for this chapter are the following:
\begin{align}
  e_+e_+^* + \left|\lambda\right|^2 e_-e_-^* &= \frac{1}{2}e^{-\Gamma t}\left[\left(1+\left|\lambda\right|^2\right)\cosh\left(\frac{\Gamma}{2}t\right)
  +\left(1-\left|\lambda\right|^2\right)\cos\left(\Delta mt\right)\right]\label{eq:result_3}\\
  e_+e_+^* \left|\lambda\right|^2 + e_-e_-^* &= \frac{1}{2}e^{-\Gamma t}\left[\left(1+\left|\lambda\right|^2\right)\cosh\left(\frac{\Gamma}{2}t\right)
  -\left(1-\left|\lambda\right|^2\right)\cos\left(\Delta mt\right)\right]\label{eq:result_4}
\end{align}
