\section{Theoretical decay rates}

After collecting all necessary terms we can now start calculating the theoretical decay rates. We start with the decays of the \Bz:
\begin{align}
  \left|\bra{f} T \ket{\Bz(t)}\right|^2 =& \left| \bra{f} T \ket{\Bz} e_+ - \frac{q}{p} \bra{f} T \ket{\Bzb}e_-\right|^2\nonumber\\
  =&\left|A_fe_+-\frac{q}{p}\overline{A}_fe_-\right|^2\nonumber\\
  =&\left|A_f\right|^2\cdot\left|e_+-\underbrace{\frac{q}{p}\frac{\overline{A}_f}{A_f}}_{\lambda}e_-\right|^2\nonumber\\
  =&\left|A_f\right|^2\left( e_+e_+^* - e_+\lambda^*e_-^*-\lambda e_-e_+^*+\left|\lambda\right|^2e_-e_-^*\right)\nonumber\\
  =&\left|A_f\right|^2\left(\underbrace{e_+e_+^* + \left|\lambda\right|^2e_-e_-^*}_{\text{\cref{eq:result_3}}}
  -\underbrace{\left(\lambda^*e_-^*e_+ + \lambda e_+^*e_-\right)}_{\text{\cref{eq:result_1}}}\right)\nonumber\\
  =&\frac{1}{2}e^{-\Gamma t}\left|A_f\right|^2\left[\left(1+\left|\lambda\right|^2\right)\cosh\left(\frac{\Delta\Gamma}{2}t\right)
  +\left(1-\left|\lambda\right|^2\right)\cos\left(\Delta mt\right)\right.\nonumber\\
  &\left.+2\mathcal{Re}\left(\lambda\right)\sinh\left(\frac{\Delta\Gamma}{2}t\right)-2\mathcal{Im}\left(\lambda\right)\sin\left(\Delta mt\right)\right]\\
  \left|\bra{\overline{f}}T\ket{\Bz(t)}\right|^2 =& \left|\bra{\overline{f}}T\ket{\Bz}e_+-\frac{q}{p}\bra{\overline{f}}T\ket{\Bzb}e_-\right|^2\nonumber\\
  =&\left|A_{\overline{f}}e_+ -\frac{q}{p}\overline{A}_{\overline{f}}e_-\right|^2\nonumber\\
  =&\left| \overline{A}_{\overline{f}} \right|^2 \cdot \left| \frac{q}{p} \right|^2 \cdot
  \left| \underbrace{\frac{p}{q}\frac{ A_{\overline{f}} }{\overline{A}_{\overline{f}}}}_{\overline{\lambda}}e_+ - e_-\right|^2\nonumber\\
  =& \left|\overline{A}_{\overline{f}}\right|^2\cdot\left|\frac{q}{p}\right|^2\cdot\left( e_+e_+^*\left|\overline{\lambda}\right|^2 +e_-e_-^*
  - \overline{\lambda^*}e_+^*e_- -\overline{\lambda}e_+e_-^*\right)\nonumber\\
  =& \left|\overline{A}_{\overline{f}}\right|^2\cdot\left|\frac{q}{p}\right|^2\cdot\left(\underbrace{e_+e_+^*\left|\overline{\lambda}\right|^2 + e_-e_-^*}_{\text{\cref{eq:result_4}}}
  -\underbrace{\left(\overline{\lambda}^*e_+^*e_- + \overline{\lambda} e_-^*e_+\right)}_{\text{\cref{eq:result_2}}}\right)\nonumber\\
  =& \frac{1}{2}e^{-\Gamma t} \left|\overline{A}_{\overline{f}}\right|^2\cdot\left|\frac{q}{p}\right|^2\left[\left(1+\left|\overline{\lambda}\right|^2\right)
  \cosh\left(\frac{\Delta\Gamma}{2}t\right)-\left(1-\left|\overline{\lambda}\right|^2\right)\cos\left(\Delta mt\right)\right.\nonumber\\
  &\left.+2\mathcal{Re}\left(\overline{\lambda}\right)\sinh\left(\frac{\Delta\Gamma}{2}t\right)
  +2\mathcal{Im}\left(\overline{\lambda}\right)\sin\left(\Delta mt\right)\right]
\end{align}
For the decays of the \Bzb the procedure is completely the same:
\begin{align}
  \left|\bra{\overline{f}} T \ket{\Bzb(t)}\right|^2
  =& \left| \bra{\overline{f}} T \ket{\Bzb} e_+ - \frac{p}{q} \bra{\overline{f}} T \ket{\Bz}e_-\right|^2\nonumber\\
  =&\left|\overline{A}_{\overline{f}}e_+ - \frac{p}{q}A_{\overline{f}}e_-\right|^2\nonumber\\
  =&\left|\overline{A}_{\overline{f}}\right|^2 \cdot
  \left| e_+ - \underbrace{\frac{p}{q}\frac{A_{\overline{f}}}{\overline{A}_{\overline{f}}}}_{\overline{\lambda}} e_- \right|^2\nonumber\\
  =&\left|\overline{A}_{\overline{f}}\right|^2
  \left( e_+e_+^* - e_+\overline{\lambda}^*e_-^*-\overline{\lambda} e_-e_+^*+\left|\overline{\lambda}\right|^2e_-e_-^*\right)\nonumber\\
  =&\left|\overline{A}_{\overline{f}}\right|^2\left(\underbrace{e_+e_+^* + \left|\overline{\lambda}\right|^2e_-e_-^*}_{\text{\cref{eq:result_3}}}
  -\underbrace{\left(e_+e_-^*\overline{\lambda}^* + e_-e_+^*\overline{\lambda} \right)}_{\text{\cref{eq:result_1}}}\right)\nonumber\\
  =&\frac{1}{2}e^{-\Gamma t}\left|\overline{A}_{\overline{f}}\right|^2\left[\left(1+\left|\overline{\lambda}\right|^2\right)
  \cosh\left(\frac{\Delta\Gamma}{2}t\right)+\left(1-\left|\overline{\lambda}\right|^2\right)\cos\left(\Delta mt\right)\right.\nonumber\\
  &\left.+2\mathcal{Re}\left(\overline{\lambda}\right)\sinh\left(\frac{\Delta\Gamma}{2}t\right)-2\mathcal{Im}\left(\overline{\lambda}\right)
  \sin\left(\Delta mt\right)\right]\\
  \left|\bra{f} T \ket{\Bzb(t)}\right|^2
  =& \left| \bra{f} T \ket{\Bzb} e_+ - \frac{p}{q} \bra{f} T \ket{\Bz}e_-\right|^2\nonumber\\
  =&\left|\overline{A}_f e_+ - \frac{p}{q} A_f e_-\right|^2\nonumber\\
  =&\left| A_f \right|^2 \cdot \left| \frac{p}{q} \right|^2 \cdot
  \left| \underbrace{\frac{q}{p}\frac{ \overline{A}_f }{ A_f }}_{\lambda} e_+ - e_-\right|^2\nonumber\\
  =& \left| A_f \right|^2 \cdot \left| \frac{p}{q} \right|^2\cdot\left( e_+e_+^*\left|\lambda\right|^2 -\lambda e_+e_-^*
  - e_-\lambda^*e_+^* + e_-e_-^*\right)\nonumber\\
  =& \left| A_f \right|^2 \cdot \left| \frac{p}{q} \right|^2\cdot\left(\underbrace{e_+e_+^*\left|\lambda\right|^2 + e_-e_-^*}_{\text{\cref{eq:result_4}}}
  -\underbrace{\left(\lambda^*e_+^*e_- + \lambda e_-^*e_+\right)}_{\text{\cref{eq:result_2}}}\right)\nonumber\\
  =&\frac{1}{2}e^{-\Gamma t}\left| A_f \right|^2 \cdot \left| \frac{p}{q} \right|^2\left[\left(1+\left|\lambda\right|^2\right)
  \cosh\left(\frac{\Delta\Gamma}{2}t\right)-\left(1-\left|\lambda\right|^2\right)\cos\left(\Delta mt\right)\right.\nonumber\\
  &\left.+2\mathcal{Re}\left(\lambda\right)\sinh\left(\frac{\Delta\Gamma}{2}t\right)
  +2\mathcal{Im}\left(\lambda\right)\sin\left(\Delta mt\right)\right]
\end{align}
So finally we try to summarise the results. First we \enquote{normalise} the decay rates in a way that the coefficient of the $\cosh$-terms is one and we
define the other coefficients as
\begin{align}
  D = \frac{2\mathcal{Re}\left(\lambda\right)}{1+\left|\lambda\right|^2} \hspace{0.5cm} &\text{and} \hspace{0.5cm}
  \overline{D} = \frac{2\mathcal{Re}\left(\overline{\lambda}\right)}{1+\left|\overline{\lambda}\right|^2}\nonumber\\
  S = \frac{2\mathcal{Im}\left(\lambda\right)}{1+\left|\lambda\right|^2} \hspace{0.5cm} &\text{and} \hspace{0.5cm}
  \overline{S} = \frac{2\mathcal{Im}\left(\overline{\lambda}\right)}{1+\left|\overline{\lambda}\right|^2}\nonumber\\
  C = \frac{1-\left|\lambda\right|^2}{1+\left|\lambda\right|^2} \hspace{0.5cm} &\text{and} \hspace{0.5cm}
  \overline{C} = \frac{1-\left|\overline{\lambda}\right|^2}{1+\left|\overline{\lambda}\right|^2}\nonumber
\end{align}
The four theoretical decay rates are then:
\begin{align}
  \Gamma\left(\Bz\to f\right) &= \frac{1}{2}e^{-\Gamma t}\left| A_f \right|^2 \left(1+\left|\lambda\right|^2\right) \cdot \left[
  \cosh\left(\frac{\Delta\Gamma}{2}t\right)+D\sinh\left(\frac{\Delta\Gamma}{2}t\right)+C\cos\left(\Delta mt\right)
  -S\sin\left(\Delta mt\right)\right] \label{eq:theodecrate1}\\
  \Gamma\left(\Bz\to \overline{f}\right) &= \frac{1}{2}e^{-\Gamma t}\left| \overline{A}_{\overline{f}} \right|^2
  \left(1+\left|\overline{\lambda}\right|^2\right) \left|\frac{q}{p}\right|^2
  \left[\cosh\left(\frac{\Delta\Gamma}{2}t\right)+\overline{D}\sinh\left(\frac{\Delta\Gamma}{2}t\right)
  -\overline{C}\cos\left(\Delta mt\right)+\overline{S}\sin\left(\Delta mt\right)\right]\label{eq:theodecrate2}\\
  \Gamma\left(\Bzb\to \overline{f}\right) &= \frac{1}{2}e^{-\Gamma t}\left| \overline{A}_{\overline{f}} \right|^2
  \left(1+\left|\overline{\lambda}\right|^2\right)
  \left[\cosh\left(\frac{\Delta\Gamma}{2}t\right)+\overline{D}\sinh\left(\frac{\Delta\Gamma}{2}t\right)
  +\overline{C}\cos\left(\Delta mt\right)-\overline{S}\sin\left(\Delta mt\right)\right]\label{eq:theodecrate3}\\
  \Gamma\left(\Bzb\to f\right) &= \frac{1}{2}e^{-\Gamma t}\left| A_f \right|^2
  \left(1+\left|\lambda\right|^2\right) \left|\frac{p}{q}\right|^2
  \left[\cosh\left(\frac{\Delta\Gamma}{2}t\right)+D\sinh\left(\frac{\Delta\Gamma}{2}t\right)
  -C\cos\left(\Delta mt\right)+S\sin\left(\Delta mt\right)\right]\label{eq:theodecrate4}
\end{align}

\subsection{HFLAV convention}
\label{sec:HFLAVconv}

The heavy flavor averaging group (HFLAV) defined a convention in which to write down the decay rate equations and thus following
the \CP coefficients. Compared to \cref{eq:theodecrate1}, \cref{eq:theodecrate2}, \cref{eq:theodecrate3} and \cref{eq:theodecrate4}
mainly some signs are moved from the equations into the definitions of the \CP coefficients. Beside these \enquote{sign-movements}
the decay width difference is defined opposite compared to \cref{eq:defdecratewidth}, while the mass difference (\cref{eq:defmassdiff})
between the mass eigenstates is defined in the same way:
\begin{align}
    \Delta m_{\text{HFLAV}} = m_H - m_L \hspace{0.5cm} &\text{and} \hspace{0.5cm} m = \frac{1}{2}\left(m_H+ m_L\right)\\
    \Delta \Gamma_{\text{HFLAV}} = \Gamma_L - \Gamma_H \hspace{0.5cm} &\text{and} \hspace{0.5cm} \Gamma = \frac{1}{2}\left(\Gamma_H + \Gamma_L\right)
\end{align}

Doing all the mentioned changes the theoretical decay rates come out as follows:
\begin{align}
  \Gamma\left(\Bz\to f\right) &\propto e^{-\Gamma t} \cdot \left[
  \cosh\left(\frac{\DG_{\scaleto{\text{HFLAV}}{4pt}}}{2}t\right)+D\sinh\left(\frac{\DG_{\scaleto{\text{HFLAV}}{4pt}}}{2}t\right)
  +C\cos\left(\dm_{\scaleto{\text{HFLAV}}{4pt}} t\right)-S\sin\left(\dm_{\scaleto{\text{HFLAV}}{4pt}} t\right)\right] \label{eq:theodecrateHFLAV1}\\
  \Gamma\left(\Bz\to \overline{f}\right) &\propto e^{-\Gamma t}
  \left[\cosh\left(\frac{\DG_{\scaleto{\text{HFLAV}}{4pt}}}{2}t\right)+\overline{D}\sinh\left(\frac{\DG_{\scaleto{\text{HFLAV}}{4pt}}}{2}t\right)
  +\overline{C}\cos\left(\dm_{\scaleto{\text{HFLAV}}{4pt}} t\right)
  -\overline{S}\sin\left(\dm_{\scaleto{\text{HFLAV}}{4pt}} t\right)\right]\label{eq:theodecrateHFLAV2}\\
  \Gamma\left(\Bzb\to \overline{f}\right) &\propto e^{-\Gamma t}
  \left[\cosh\left(\frac{\DG_{\scaleto{\text{HFLAV}}{4pt}}}{2}t\right)+\overline{D}\sinh\left(\frac{\DG_{\scaleto{\text{HFLAV}}{4pt}}}{2}t\right)
  -\overline{C}\cos\left(\dm_{\scaleto{\text{HFLAV}}{4pt}} t\right)
  +\overline{S}\sin\left(\dm_{\scaleto{\text{HFLAV}}{4pt}} t\right)\right]\label{eq:theodecrateHFLAV3}\\
  \Gamma\left(\Bzb\to f\right) &\propto e^{-\Gamma t}
  \left[\cosh\left(\frac{\DG_{\scaleto{\text{HFLAV}}{4pt}}}{2}t\right)+D\sinh\left(\frac{\DG_{\scaleto{\text{HFLAV}}{4pt}}}{2}t\right)
  -C\cos\left(\dm_{\scaleto{\text{HFLAV}}{4pt}} t\right)
  +S\sin\left(\dm_{\scaleto{\text{HFLAV}}{4pt}} t\right)\right]\label{eq:theodecrateHFLAV4}
\end{align}
with the following \CP coefficients:
\begin{align}
  D = -\frac{2\mathcal{Re}\left(\lambda\right)}{1+\left|\lambda\right|^2} \hspace{0.5cm} &\text{and} \hspace{0.5cm}
  \overline{D} = -\frac{2\mathcal{Re}\left(\overline{\lambda}\right)}{1+\left|\overline{\lambda}\right|^2}\nonumber\\
  S = \frac{2\mathcal{Im}\left(\lambda\right)}{1+\left|\lambda\right|^2} \hspace{0.5cm} &\text{and} \hspace{0.5cm}
  \overline{S} = -\frac{2\mathcal{Im}\left(\overline{\lambda}\right)}{1+\left|\overline{\lambda}\right|^2}\nonumber\\
  C = \frac{1-\left|\lambda\right|^2}{1+\left|\lambda\right|^2} \hspace{0.5cm} &\text{and} \hspace{0.5cm}
  \overline{C} = -\frac{1-\left|\overline{\lambda}\right|^2}{1+\left|\overline{\lambda}\right|^2}\nonumber
\end{align}
